theories/interop/gctoken.v
@@ -58,13 +58,14 @@ Context `{!wrapperGCtokG Σ}.
 Definition GC (θ : addr_map) : iProp Σ :=
   ∃ (ζ : lstore) (χ : lloc_map) (σMLvirt : store)
     (roots_s : list $ gset addr) (roots_fm : list roots_map) (roots_gm : roots_map)
-    (roots_f : list gname),
+    (roots_f : list gname) (roots_lm : gmap gname unit),
     "GCζ" ∷ ghost_var wrapperG_γζ (1/2) ζ
   ∗ "GCχ" ∷ ghost_var wrapperG_γχ (1/2) χ
   ∗ "GCθ" ∷ ghost_var wrapperG_γθ (1/2) θ
   ∗ "GCHGH" ∷ HGH χ (Some σMLvirt) ζ
   ∗ "GCinit" ∷ ghost_var wrapperG_γat_init (1/2) false
   ∗ "GCroots" ∷ ghost_var wrapperG_γroots_set (1/2) roots_s
+  ∗ "GCrootslive" ∷ ghost_map_auth wrapperG_γroots_live_map 1 roots_lm
   ∗ "GCrootsf" ∷ ghost_var wrapperG_γroots_frame (1/2) roots_f
   ∗ "GCrootsg" ∷ ghost_map_auth wrapperG_γroots_global_map 1 roots_gm
   ∗ "GCrootsm" ∷ ([∗ list] f; r ∈ roots_f; roots_fm, ghost_map_auth f (1/2) r)
@@ -72,6 +73,8 @@ Definition GC (θ : addr_map) : iProp Σ :=
                    ([∗ map] a ↦ v ∈ r, ∃ w, a ↦C w ∗ ⌜repr_lval θ v w⌝))
   ∗ "%Hrootsdom" ∷ ⌜map dom (roots_fm++[roots_gm]) = roots_s⌝
   ∗ "%Hrootslive" ∷ ⌜roots_are_live θ (roots_fm++[roots_gm])⌝
+  ∗ "%Hlocalrootslive" ∷ ⌜dom roots_lm = list_to_set roots_f⌝
+  ∗ "%Hlocalnodup" ∷ ⌜NoDup roots_f⌝
   ∗ "%HGCOK" ∷ ⌜GC_correct ζ θ⌝.
 
 Definition at_init := ghost_var wrapperG_γat_init (1/2) true.
