theories/interop/wp_prims/alloc_foreign.v
@@ -71,7 +71,7 @@ Proof using.
   iApply ("Cont" $! θC' γ with "[-]"); try done.
   iFrame. iSplit; last by eauto.
   rewrite /GC /named.
-  iExists _, _, σMLvirt, _, _, _, _. iFrame; eauto.
+  iExists _, _, σMLvirt, _, _, _, _, _. iFrame; eauto.
 Admitted.
 
 End Laws.
